#MHV4U #Homework 
# Unit 1

## 1.1 

1. 
	1. $2 \sqrt3 +4$ 
	2. $\sqrt3-\sqrt2$
	3. $-2\sqrt3+\sqrt2$
	4. $3\sqrt3-\sqrt2$
	5. $\sqrt2+\sqrt5$\
	   6. $-\sqrt5+2\sqrt2$
2.  .
	1. $\frac{\sqrt6+\sqrt10}{2}$
	2. $\sqrt6-3$
	3. $\frac{4+\sqrt6}{2}$
	4. $\frac{3\sqrt10-2}{4}$
3. .
	1. 
4. 

## 1.2

$$
\begin{align}
\frac{(5+h)^3-125}{h}\\
\frac{(5+h)(5+h)(5+h)-125}{h}\\
\frac{(h^2+10h+25)(5+h)-125}{h}\\
\frac{(h^2+15h^2+75h+125)-125}{h}\\
\frac{h^3+15h^2+75h}{h}\\
\end{align}
$$
## 1.3

1. it's at rest at 0 seconds and at 4 seconds 
5. speed is not a vector
6. technically no 
7. 
	1. 5m/s, -15, -40 m/s respectively  
	2. 55 m/s
	3. $$\begin{align}v(t)&=\frac{s(t+h)-s(t)}{h}\\v(t)&=\frac{320-5(3-h)^2-(320-5(3)^2)}{h}\\v(t)&=\frac{30h-5h^2}{h}\\v(t)&=\frac{h(30-5h)}{h}\\v(t)&=\lim_{x\to0}30-5h\\v(t)&=30\end{align}$$
9. 
	1. 15
	2. $$\begin{align}t(x)&=\frac{f(x+h)-f(x)}{h}\\t(x)&=\frac{20(2+h)-(2+h)^2-(20(2)-2^2)}{h}\\t(x)&=\frac{16h-h^2}{h}\\t(x)&=\frac{h(16-h)}{h}\\t(x)&=\lim_{x\to0}16-h\\t(x)&=16\end{align}$$

## 1.4
1. 
	1. $\frac{72}{99}^-$ 
	2. $\pi^-$
4. 
	1. -5
	2. 10
	3. 100
	4. -8
	5. 4
	6. 8
6. 
	1. 0
	2. 2
	3. -1
	4. 2
7. 
	1. 2
	2. 1
	3. DNE
10. 
	1. 0
	2. 0 
	3. 5
	4. $-\frac{1}{2}$ 
	5. $\frac15$
	6. DNE
13.  m=-1 b=3
14. a=3 b=2 c=0
	## 1.5

3. yep, if both are the same limit exists, if not it doesn't 
4. 
	1. 1
	2. 1
	3. $\frac{100}{9}$ 
	4. $5\pi^3$
	5. 2
	6. 3
7. 
	1. 4
	2. 1
	3. 27
	4. $$\begin{align}&\lim_{x\to0}\frac{\sqrt{7-x}-\sqrt{7+x}}{x}\\&\lim_{x\to0}\frac{\sqrt{7-x}-\sqrt{7+x}}{x}\times\frac{\sqrt{7-x}+\sqrt{7+x}}{\sqrt{7-x}+\sqrt{7+x}}\\&\lim_{x\to0}\frac{2x}{x(\sqrt{7-x}+\sqrt{7+x})}\\&\frac2{2\sqrt7}\\&\frac1{\sqrt7}\end{align}$$
8. 
	1. let a be $\sqrt[3]x$ $$\begin{align}&\lim_{a\to2}\frac{a-2}{a^3-8}\\&\frac{a-2}{a-2(a^2+2a+4)}\\&\frac{1}{16}\end{align}$$
	2. let a be $\sqrt[3]x$ $$$$
9. A
## 1.6

2. no holes no jump no VA
3. point jump infinite
4. 1
	1. hole at x=3
	2. 
	3. VA at x=-1


$$
\begin{align}
&\lim_{x\to2}\frac{\sqrt{6-x}-2}{\sqrt{3-x}-1}\times\frac{\sqrt{3-x}+1}{\sqrt{3-x}+1}\\
&\lim_{x\to2}\frac{(\sqrt{6-x}-2)(\sqrt{3-x}+1)}{3-x-1}\times\frac{\sqrt{6-x}+2}{\sqrt{6-x}+2}\\
&\lim_{x\to2}\frac{(2-x)(\sqrt{3-x}+1)}{(2-x)(\sqrt{6-x}+2)}\\
&=\frac{(\sqrt{3-2}+1)}{(\sqrt{6-2}+2)}\\
&=\frac{2}{4}\\
&=\frac12
\end{align}
$$
